2.dfy
@@ -1,7 +1,14 @@
-// map function over an array. checks which elements are larger than a given x, substitutes those by their multiplication with x
-// return the amount of values bigger than x
+/* I interpret this problem statement in two different ways:
+     1: map function over an array. checks which elements are larger than a given x, substitutes those by their multiplication with x
+        then, return the amount of values bigger than x
 
-method mapmult(arr: array?<int>, x: int) returns (count: nat)
+     2: map function over an array. returns 'n', the count of all elements larger than a given x
+        those elements should be substituted by x * n
+
+  mapmult1 represents interpretation 1, mapmult2 represents interpretation 2.
+*/
+
+method mapmult1(arr: array?<int>, x: int) returns (count: nat)
   requires arr != null
   modifies arr
 
@@ -54,5 +61,75 @@ method mapmult(arr: array?<int>, x: int) returns (count: nat)
     }
 
     i := i + 1;
+  }
+}
+
+method mapmult2(arr: array?<int>, x: int) returns (count: nat)
+  requires arr != null
+  modifies arr
+
+  // if a value at a given position in the array is:
+  // - bigger than the given x, becomes count * x
+  // - smaller or equal than the given x, stays the same
+  ensures forall i :: 0 <= i < arr.Length ==>
+                        (old(arr[i]) > x ==> arr[i] == count * x) &&
+                        (old(arr[i]) <= x ==> arr[i] == old(arr[i]))
+
+  // the return value, count, will be exactly the number of values bigger than x in the
+  // starting array
+  ensures count == | (set i | 0 <= i < arr.Length && old(arr[i]) > x) |
+{
+  count := 0;
+  var i := 0;
+
+  while (i < arr.Length)
+    decreases arr.Length - i
+
+    // only valid indices
+    invariant 0 <= i <= arr.Length
+
+    // dafny is not smart enough to prove this by itself, so we need the asserts
+    // inside the if and else blocks
+    invariant count == | (set j | 0 <= j < i && old(arr[j]) > x) |
+
+  {
+    if (arr[i] > x) {
+      // proving to dafny that:
+      // - the new set will include j = i
+      // - so the count will increase by exactly 1
+      assert old(arr[i]) > x;
+      assert 0 <= i < arr.Length;
+      assert (set j | 0 <= j < i + 1 && old(arr[j]) > x) == (set j | 0 <= j < i && old(arr[j]) > x) + {i};
+
+      count := count + 1;
+    } else {
+      // here the set doesn't change because arr[i] is not > x
+      assert old(arr[i]) <= x;
+      assert (set j | 0 <= j < i + 1 && old(arr[j]) > x) == (set j | 0 <= j < i && old(arr[j]) > x);
+    }
+
+    i := i + 1;
+  }
+
+  var k := 0;
+  while (k < arr.Length)
+    decreases arr.Length - k
+
+    // only valid indices
+    invariant 0 <= k <= arr.Length
+
+    // the invariant is the same as the post condition, up until i (the current iterator)
+    invariant forall j :: 0 <= j < k ==>
+                            (old(arr[j]) > x ==> arr[j] == count * x) &&
+                            (old(arr[j]) <= x ==> arr[j] == old(arr[j]))
+
+    // all of the other positions are still unchanged
+    invariant forall j :: k <= j < arr.Length ==> arr[j] == old(arr[j])
+  {
+    if (arr[k] > x) {
+      arr[k] := count * x;
+    }
+
+    k := k + 1;
   }
 }
